Add a arith_shift_right_rwt theorem.

compiler/bootstrap/translation/to_word64ProgScript.sml
@@ -98,6 +98,23 @@ val shift_right_rwt = Q.prove(
   \\ qpat_x_assum `!n. P` (assume_tac o GSYM)
   \\ fs [])
 
+val arith_shift_right_def = Define`
+  arith_shift_right (a : 'a word) n =
+  if n = 0 then a
+  else if (a = 0w) \/ n > dimindex(:'a) /\ ~word_msb a then 0w
+  else if (a = -1w) \/ n > dimindex(:'a) /\ word_msb a then -1w
+  else if n > 32 then arith_shift_right (a >> 32) (n - 32)
+  else if n > 16 then arith_shift_right (a >> 16) (n - 16)
+  else if n > 8 then arith_shift_right (a >> 8) (n - 8)
+  else arith_shift_right (a >> 1) (n - 1)`
+
+val arith_shift_right_rwt = Q.prove(
+  `!a n. a >> n = arith_shift_right a n`,
+  completeInduct_on `n`
+  \\ rw [Once arith_shift_right_def]
+  \\ qpat_x_assum `!n. P` (assume_tac o GSYM)
+  \\ fs [SIMP_RULE (srw_ss()) [] wordsTheory.ASR_UINT_MAX])
+
 val _ = translate (shift_left_def |> conv64)
 val _ = translate (shift_right_def |> spec64 |> CONV_RULE fcpLib.INDEX_CONV)
 
